Finish eval_correct proof

src/hls/HTLPargen.v
@@ -33,6 +33,11 @@ Require Import vericert.hls.Verilog.
 Require Import vericert.hls.Gible.
 Require Import vericert.hls.GiblePar.
 Require Import vericert.hls.Predicate.
+Require Import vericert.common.Errormonad.
+Import ErrorMonad.
+Import ErrorMonadExtra.
+
+#[local] Open Scope monad_scope.
 
 #[local] Hint Resolve AssocMap.gempty : htlh.
 #[local] Hint Resolve AssocMap.gso : htlh.
@@ -40,61 +45,13 @@ Require Import vericert.hls.Predicate.
 #[local] Hint Resolve Ple_refl : htlh.
 #[local] Hint Resolve Ple_succ : htlh.
 
-Record state: Type := mkstate {
-  st_st : reg;
-  st_freshreg: reg;
-  st_freshstate: node;
-  st_scldecls: AssocMap.t (option io * scl_decl);
-  st_arrdecls: AssocMap.t (option io * arr_decl);
-  st_datapath: datapath;
+Record control_regs: Type := mk_control_regs {
+  ctrl_st : reg;
+  ctrl_stack : reg;
+  ctrl_preg : reg;
+  ctrl_fin : reg;
+  ctrl_return : reg;
 }.
-
-Definition init_state (st : reg) : state :=
-  mkstate st
-          1%positive
-          1%positive
-          (AssocMap.empty (option io * scl_decl))
-          (AssocMap.empty (option io * arr_decl))
-          (AssocMap.empty stmnt).
-
-Module HTLState <: State.
-
-  Definition st := state.
-
-  Inductive st_incr: state -> state -> Prop :=
-    state_incr_intro:
-      forall (s1 s2: state),
-        st_st s1 = st_st s2 ->
-        Ple s1.(st_freshreg) s2.(st_freshreg) ->
-        Ple s1.(st_freshstate) s2.(st_freshstate) ->
-        (forall n,
-            s1.(st_datapath)!n = None \/ s2.(st_datapath)!n = s1.(st_datapath)!n) ->
-        st_incr s1 s2.
-  #[export] Hint Constructors st_incr : htlh.
-
-  Definition st_prop := st_incr.
-  #[export] Hint Unfold st_prop : htlh.
-
-  Lemma st_refl : forall s, st_prop s s. Proof. auto with htlh. Qed.
-
-  Lemma st_trans :
-    forall s1 s2 s3, st_prop s1 s2 -> st_prop s2 s3 -> st_prop s1 s3.
-  Proof.
-    intros. inv H. inv H0. apply state_incr_intro; eauto using Ple_trans; intros; try congruence.
-    - destruct H4 with n; destruct H7 with n; intuition congruence.
-  Qed.
-
-End HTLState.
-Export HTLState.
-
-Module HTLMonad := Statemonad(HTLState).
-Export HTLMonad.
-
-Module HTLMonadExtra := Monad.MonadExtra(HTLMonad).
-Import HTLMonadExtra.
-Export MonadNotation.
-
-#[local] Open Scope monad_scope.
 
 Definition pred_lit (preg: reg) (pred: predicate) :=
   Vrange preg (Vlit (posToValue pred)) (Vlit (posToValue pred)).
@@ -133,62 +90,6 @@ Definition state_goto (preg: reg) (p: option pred_op) (st : reg) (n : node) : st
 Definition state_cond (preg: reg) (p: option pred_op) (st : reg) (c : expr) (n1 n2 : node) : stmnt :=
   translate_predicate Vblock preg p (Vvar st) (Vternary c (posToExpr n1) (posToExpr n2)).
 
-Definition check_empty_node_datapath:
-  forall (s: state) (n: node), { s.(st_datapath)!n = None } + { True }.
-Proof.
-  intros. case (s.(st_datapath)!n); tauto.
-Defined.
-
-Definition append_instr (n : node) (st : stmnt) (d : datapath) : datapath :=
-  match AssocMap.get n d with 
-  | Some st' => AssocMap.set n (Vseq st' st) d
-  | None => AssocMap.set n st d
-  end.
-
-Lemma declare_reg_state_incr :
-  forall i s r sz,
-    st_incr s
-    (mkstate
-       s.(st_st)
-       s.(st_freshreg)
-       s.(st_freshstate)
-       (AssocMap.set r (i, VScalar sz) s.(st_scldecls))
-       s.(st_arrdecls)
-       s.(st_datapath)).
-Proof. Admitted.
-
-Definition declare_reg (i : option io) (r : reg) (sz : nat) : mon unit :=
-  fun s => OK tt (mkstate
-                s.(st_st)
-                s.(st_freshreg)
-                s.(st_freshstate)
-                (AssocMap.set r (i, VScalar sz) s.(st_scldecls))
-                s.(st_arrdecls)
-                s.(st_datapath))
-              (declare_reg_state_incr i s r sz).
-
-Lemma declare_arr_state_incr :
-  forall i s r sz ln,
-    st_incr s
-    (mkstate
-       s.(st_st)
-       s.(st_freshreg)
-       s.(st_freshstate)
-       s.(st_scldecls)
-       (AssocMap.set r (i, VArray sz ln) s.(st_arrdecls))
-       s.(st_datapath)).
-Proof. Admitted.
-
-Definition declare_arr (i : option io) (r : reg) (sz : nat) (ln : nat) : mon unit :=
-  fun s => OK tt (mkstate
-                s.(st_st)
-                s.(st_freshreg)
-                s.(st_freshstate)
-                s.(st_scldecls)
-                (AssocMap.set r (i, VArray sz ln) s.(st_arrdecls))
-                s.(st_datapath))
-              (declare_arr_state_incr i s r sz ln).
-
 Definition nonblock (dst : reg) (e : expr) := Vnonblock (Vvar dst) e.
 Definition block (dst : reg) (e : expr) := Vblock (Vvar dst) e.
 
@@ -201,15 +102,17 @@ Definition boplit (op : binop) (r : reg) (l : Integers.int) : expr :=
 Definition boplitz (op: binop) (r: reg) (l: Z) : expr :=
   Vbinop op (Vvar r) (Vlit (ZToValue l)).
 
+Definition error {A} m := @Errors.Error A (Errors.msg m).
+
 Definition translate_comparison (c : Integers.comparison) (args : list reg) : Errors.res expr :=
   match c, args with
-  | Integers.Ceq, r1::r2::nil => Errors.OK (bop Veq r1 r2)
-  | Integers.Cne, r1::r2::nil => Errors.OK (bop Vne r1 r2)
-  | Integers.Clt, r1::r2::nil => Errors.OK (bop Vlt r1 r2)
-  | Integers.Cgt, r1::r2::nil => Errors.OK (bop Vgt r1 r2)
-  | Integers.Cle, r1::r2::nil => Errors.OK (bop Vle r1 r2)
-  | Integers.Cge, r1::r2::nil => Errors.OK (bop Vge r1 r2)
-  | _, _ => Errors.Error (Errors.msg "Htlgen: comparison instruction not implemented: other")
+  | Integers.Ceq, r1::r2::nil => ret (bop Veq r1 r2)
+  | Integers.Cne, r1::r2::nil => ret (bop Vne r1 r2)
+  | Integers.Clt, r1::r2::nil => ret (bop Vlt r1 r2)
+  | Integers.Cgt, r1::r2::nil => ret (bop Vgt r1 r2)
+  | Integers.Cle, r1::r2::nil => ret (bop Vle r1 r2)
+  | Integers.Cge, r1::r2::nil => ret (bop Vge r1 r2)
+  | _, _ => error "Htlpargen: comparison instruction not implemented: other"
   end.
 
 Definition translate_comparison_imm (c : Integers.comparison) (args : list reg) (i: Integers.int)
@@ -221,7 +124,7 @@ Definition translate_comparison_imm (c : Integers.comparison) (args : list reg) 
   | Integers.Cgt, r1::nil => Errors.OK (boplit Vgt r1 i)
   | Integers.Cle, r1::nil => Errors.OK (boplit Vle r1 i)
   | Integers.Cge, r1::nil => Errors.OK (boplit Vge r1 i)
-  | _, _ => Errors.Error (Errors.msg "Htlgen: comparison_imm instruction not implemented: other")
+  | _, _ => error "Htlpargen: comparison_imm instruction not implemented: other"
   end.
 
 Definition translate_comparisonu (c : Integers.comparison) (args : list reg) : Errors.res expr :=
@@ -230,7 +133,7 @@ Definition translate_comparisonu (c : Integers.comparison) (args : list reg) : E
   | Integers.Cgt, r1::r2::nil => Errors.OK (bop Vgtu r1 r2)
   | Integers.Cle, r1::r2::nil => Errors.OK (bop Vleu r1 r2)
   | Integers.Cge, r1::r2::nil => Errors.OK (bop Vgeu r1 r2)
-  | _, _ => Errors.Error (Errors.msg "Htlgen: comparison instruction not implemented: other")
+  | _, _ => Errors.Error (Errors.msg "Htlpargen: comparison instruction not implemented: other")
   end.
 
 Definition translate_comparison_immu (c : Integers.comparison) (args : list reg) (i: Integers.int)
@@ -240,7 +143,7 @@ Definition translate_comparison_immu (c : Integers.comparison) (args : list reg)
   | Integers.Cgt, r1::nil => Errors.OK (boplit Vgtu r1 i)
   | Integers.Cle, r1::nil => Errors.OK (boplit Vleu r1 i)
   | Integers.Cge, r1::nil => Errors.OK (boplit Vgeu r1 i)
-  | _, _ => Errors.Error (Errors.msg "Htlgen: comparison_imm instruction not implemented: other")
+  | _, _ => Errors.Error (Errors.msg "Htlpargen: comparison_imm instruction not implemented: other")
   end.
 
 Definition translate_condition (c : Op.condition) (args : list reg) : Errors.res expr :=
@@ -249,9 +152,9 @@ Definition translate_condition (c : Op.condition) (args : list reg) : Errors.res
   | Op.Ccompu c, _ => translate_comparisonu c args
   | Op.Ccompimm c i, _ => translate_comparison_imm c args i
   | Op.Ccompuimm c i, _ => translate_comparison_immu c args i
-  | Op.Cmaskzero n, _ => Errors.Error (Errors.msg "Htlgen: condition instruction not implemented: Cmaskzero")
-  | Op.Cmasknotzero n, _ => Errors.Error (Errors.msg "Htlgen: condition instruction not implemented: Cmasknotzero")
-  | _, _ => Errors.Error (Errors.msg "Htlgen: condition instruction not implemented: other")
+  | Op.Cmaskzero n, _ => Errors.Error (Errors.msg "Htlpargen: condition instruction not implemented: Cmaskzero")
+  | Op.Cmasknotzero n, _ => Errors.Error (Errors.msg "Htlpargen: condition instruction not implemented: Cmasknotzero")
+  | _, _ => Errors.Error (Errors.msg "Htlpargen: condition instruction not implemented: other")
   end.
 
 Definition check_address_parameter_signed (p : Z) : bool :=
@@ -299,8 +202,8 @@ Definition translate_instr (op : Op.operation) (args : list reg) : Errors.res ex
   | Op.Osub, r1::r2::nil => Errors.OK (bop Vsub r1 r2)
   | Op.Omul, r1::r2::nil => Errors.OK (bop Vmul r1 r2)
   | Op.Omulimm n, r::nil => Errors.OK (boplit Vmul r n)
-  | Op.Omulhs, r1::r2::nil => Errors.Error (Errors.msg "Htlgen: Instruction not implemented: mulhs")
-  | Op.Omulhu, r1::r2::nil => Errors.Error (Errors.msg "Htlgen: Instruction not implemented: mulhu")
+  | Op.Omulhs, r1::r2::nil => Errors.Error (Errors.msg "Htlpargen: Instruction not implemented: mulhs")
+  | Op.Omulhu, r1::r2::nil => Errors.Error (Errors.msg "Htlpargen: Instruction not implemented: mulhu")
   | Op.Odiv, r1::r2::nil => Errors.OK (bop Vdiv r1 r2)
   | Op.Odivu, r1::r2::nil => Errors.OK (bop Vdivu r1 r2)
   | Op.Omod, r1::r2::nil => Errors.OK (bop Vmod r1 r2)
@@ -322,7 +225,7 @@ Definition translate_instr (op : Op.operation) (args : list reg) : Errors.res ex
                   (Vbinop Vshru (Vvar r) (Vlit n)))
   | Op.Oshru, r1::r2::nil => Errors.OK (bop Vshru r1 r2)
   | Op.Oshruimm n, r::nil => Errors.OK (boplit Vshru r n)
-  | Op.Ororimm n, r::nil => Errors.Error (Errors.msg "Htlgen: Instruction not implemented: Ororimm")
+  | Op.Ororimm n, r::nil => Errors.Error (Errors.msg "Htlpargen: Instruction not implemented: Ororimm")
   (*Errors.OK (Vbinop Vor (boplit Vshru r (Integers.Int.modu n (Integers.Int.repr 32)))
                                         (boplit Vshl r (Integers.Int.sub (Integers.Int.repr 32) (Integers.Int.modu n (Integers.Int.repr 32)))))*)
   | Op.Oshldimm n, r::nil => Errors.OK (Vbinop Vor (boplit Vshl r n) (boplit Vshr r (Integers.Int.sub (Integers.Int.repr 32) n)))
@@ -331,7 +234,7 @@ Definition translate_instr (op : Op.operation) (args : list reg) : Errors.res ex
     do tc <- translate_condition c rl;
     Errors.OK (Vternary tc (Vvar r1) (Vvar r2))
   | Op.Olea a, _ => translate_eff_addressing a args
-  | _, _ => Errors.Error (Errors.msg "Htlgen: Instruction not implemented: other")
+  | _, _ => Errors.Error (Errors.msg "Htlpargen: Instruction not implemented: other")
   end.
 
 Definition translate_arr_access (mem : AST.memory_chunk) (addr : Op.addressing)
@@ -393,8 +296,6 @@ Definition translate_cfi (fin rtrn state preg: reg) p (cfi: cf_instr)
     Errors.Error (Errors.msg "HTLPargen: RBbuildin not supported.")
   end.
 
-Definition dfltp {A} (p: option (@Predicate.pred_op A)) := Option.default Ptrue p.
-
 Definition transf_instr (fin rtrn stack state preg: reg) 
            (dc: pred_op * stmnt) (i: instr)
            : Errors.res (pred_op * stmnt) :=
@@ -423,20 +324,17 @@ Definition transf_instr (fin rtrn stack state preg: reg)
     Errors.OK (Pand curr_p (negate (dfltp p)), Vseq d d_stmnt)
   end.
 
-Definition fold_leftE {A B} (f: A -> B -> Errors.res A) (l: list B) (el: A): Errors.res A :=
-  fold_left (fun a b => do a' <- a; f a' b) l (Errors.OK el).
-
 Definition transf_chained_block (fin rtrn stack state preg: reg)
            (dc: @pred_op positive * stmnt)
            (block: list instr)
            : Errors.res (pred_op * stmnt) :=
-  fold_leftE (transf_instr fin rtrn stack state preg) block dc.
+  mfold_left (transf_instr fin rtrn stack state preg) block (ret dc).
 
 Definition transf_parallel_block (fin rtrn stack state preg: reg)
            (dc: @pred_op positive * stmnt)
            (block: list (list instr))
            : Errors.res (pred_op * stmnt) :=
-  fold_leftE (transf_chained_block fin rtrn stack state preg) block dc.
+  mfold_left (transf_chained_block fin rtrn stack state preg) block (ret dc).
 
 Definition transf_parallel_full_block (fin rtrn stack state preg: reg)
            (dc: node * @pred_op positive * datapath)
@@ -457,85 +355,14 @@ Definition transf_seq_block (fin rtrn stack state preg: reg)
            (d: datapath) (n: node)
            (block: list (list (list instr)))
            : Errors.res datapath :=
-  do res <- fold_leftE
-    (transf_parallel_full_block fin rtrn stack state preg) block (n, Ptrue, d);
+  do res <- mfold_left
+    (transf_parallel_full_block fin rtrn stack state preg) block (ret (n, Ptrue, d));
   let '(_, _, d') := res in
   Errors.OK d'.
 
-#[local] Close Scope error_monad_scope.
-#[local] Open Scope monad_scope.
-
-Program Definition transf_seq_blockM (fin rtrn stack preg: reg) (ni: node * ParBB.t): mon unit :=
-  fun st =>
+Definition transf_seq_blockM (ctrl: control_regs) (d: datapath) (ni: node * ParBB.t): res datapath :=
     let (n, i) := ni in
-    match transf_seq_block fin rtrn stack st.(st_st) preg st.(st_datapath) n i with
-    | Errors.OK d => 
-      OK tt (mkstate st.(st_st)
-             st.(st_freshreg)
-             st.(st_freshstate)
-             st.(st_scldecls)
-             st.(st_arrdecls)
-             d) _
-    | Errors.Error m => Error m
-    end.
-Next Obligation.
-admit.
-Admitted.
-
-Definition declare_regs (i: instr): mon unit :=
-  match i with
-  | RBop _ _ _ d => declare_reg None d 32
-  | RBload _ _ _ _ d => declare_reg None d 32
-  | _ => ret tt
-  end.
-
-Definition declare_all_regs (ni: node * ParBB.t): mon unit :=
-  let (n, i) := ni in
-  ParBB.foldl _ (fun (st_f: mon unit) i => do _tt <- st_f; declare_regs i) i (ret tt).
-
-Lemma create_reg_state_incr:
-  forall s sz i,
-    st_incr s (mkstate
-         s.(st_st)
-         (Pos.succ (st_freshreg s))
-         (st_freshstate s)
-         (AssocMap.set s.(st_freshreg) (i, VScalar sz) s.(st_scldecls))
-         s.(st_arrdecls)
-         (st_datapath s)).
-Proof. constructor; simpl; auto with htlh. Qed.
-
-Definition create_reg (i : option io) (sz : nat) : mon reg :=
-  fun s => let r := s.(st_freshreg) in
-           OK r (mkstate
-                   s.(st_st)
-                   (Pos.succ r)
-                   (st_freshstate s)
-                   (AssocMap.set s.(st_freshreg) (i, VScalar sz) s.(st_scldecls))
-                   (st_arrdecls s)
-                   (st_datapath s))
-              (create_reg_state_incr s sz i).
-
-Lemma create_arr_state_incr:
-  forall s sz ln i,
-    st_incr s (mkstate
-         s.(st_st)
-         (Pos.succ (st_freshreg s))
-         (st_freshstate s)
-         s.(st_scldecls)
-         (AssocMap.set s.(st_freshreg) (i, VArray sz ln) s.(st_arrdecls))
-         (st_datapath s)).
-Proof. constructor; simpl; auto with htlh. Qed.
-
-Definition create_arr (i : option io) (sz : nat) (ln : nat) : mon (reg * nat) :=
-  fun s => let r := s.(st_freshreg) in
-           OK (r, ln) (mkstate
-                   s.(st_st)
-                   (Pos.succ r)
-                   (st_freshstate s)
-                   s.(st_scldecls)
-                   (AssocMap.set s.(st_freshreg) (i, VArray sz ln) s.(st_arrdecls))
-                   (st_datapath s))
-              (create_arr_state_incr s sz ln i).
+    transf_seq_block ctrl.(ctrl_fin) ctrl.(ctrl_return) ctrl.(ctrl_stack) ctrl.(ctrl_st) ctrl.(ctrl_preg) d n i.
 
 Definition stack_correct (sz : Z) : bool :=
   (0 <=? sz) && (sz <? Integers.Ptrofs.modulus) && (Z.modulo sz 4 =? 0).
@@ -580,61 +407,46 @@ Definition decide_order a b c d e f g h : {module_ordering a b c d e f g h} + {T
                    end; unfold module_ordering; auto.
 Defined.
 
-Definition transf_module (f: function) : mon DHTL.module.
-  refine (
+Program Definition transl_module (f: function) : res DHTL.module :=
   if stack_correct f.(fn_stacksize) then
-    do fin <- create_reg (Some Voutput) 1;
-    do rtrn <- create_reg (Some Voutput) 32;
-    do (stack, stack_len) <- create_arr None 32 (Z.to_nat (f.(fn_stacksize) / 4));
-    do start <- create_reg (Some Vinput) 1;
-    do rst <- create_reg (Some Vinput) 1;
-    do clk <- create_reg (Some Vinput) 1;
-    do preg <- create_reg None 128;
-    do _stmnt <- collectlist (transf_seq_blockM fin rtrn stack preg) (Maps.PTree.elements f.(GiblePar.fn_code));
-    do _stmnt' <- collectlist (fun r => declare_reg (Some Vinput) r 32) f.(GiblePar.fn_params);
-    do _stmnt'' <- collectlist declare_all_regs (Maps.PTree.elements f.(GiblePar.fn_code));
-    do current_state <- get;
-    match zle (Z.pos (max_pc_map current_state.(st_datapath))) Integers.Int.max_unsigned,
-          decide_order (st_st current_state) fin rtrn stack start rst clk preg,
-          max_list_dec (GiblePar.fn_params f) (st_st current_state)
+    let st := Pos.succ (max_reg_function f) in
+    let fin := Pos.succ st in
+    let rtrn := Pos.succ fin in
+    let stack := Pos.succ rtrn in
+    let start := Pos.succ stack in
+    let rst := Pos.succ start in
+    let clk := Pos.succ rst in
+    let preg := Pos.succ clk in 
+    do _stmnt <- mfold_left (transf_seq_blockM (mk_control_regs st stack preg fin rtrn)) 
+                            (Maps.PTree.elements f.(GiblePar.fn_code)) (ret (PTree.empty _));
+    match zle (Z.pos (max_pc_map _stmnt)) Integers.Int.max_unsigned,
+            decide_order st fin rtrn stack start rst clk preg,
+            max_list_dec (GiblePar.fn_params f) st
     with
     | left LEDATA, left MORD, left WFPARAMS =>
         ret (DHTL.mkmodule
            f.(GiblePar.fn_params)
-           current_state.(st_datapath)
+           _stmnt
            f.(fn_entrypoint)
-           current_state.(st_st)
+           st
            stack
-           stack_len
+           (Z.to_nat (f.(fn_stacksize) / 4))
            fin
            rtrn
            start
            rst
            clk
            preg
-           current_state.(st_scldecls)
-           current_state.(st_arrdecls)
+           (AssocMap.empty _)
+           (AssocMap.empty _)
            None
            (max_pc_wf _ LEDATA)
            MORD
            _
            WFPARAMS)
-    | _, _, _ => error (Errors.msg "More than 2^32 states.")
+    | _, _, _ => error "More than 2^32 states."
     end
-  else error (Errors.msg "Stack size misalignment.")); discriminate.
-Defined.
-
-Definition max_state (f: function) : state :=
-  let st := Pos.succ (max_reg_function f) in
-  mkstate st
-          (Pos.succ st)
-          (Pos.succ (max_pc_function f))
-          (AssocMap.set st (None, VScalar 32) (st_scldecls (init_state st)))
-          (st_arrdecls (init_state st))
-          (st_datapath (init_state st)).
-
-Definition transl_module (f : function) : Errors.res DHTL.module :=
-  run_mon (max_state f) (transf_module f).
+  else error "Stack size misalignment.".
 
 Definition transl_fundef := transf_partial_fundef transl_module.
 
