src/hls/DMemorygen.v
@@ -1,6 +1,6 @@
 (*
  * Vericert: Verified high-level synthesis.
- * Copyright (C) 2021 Yann Herklotz <yann@yannherklotz.com>
+ * Copyright (C) 2021-2023 Yann Herklotz <yann@yannherklotz.com>
  *
  * This program is free software: you can redistribute it and/or modify
  * it under the terms of the GNU General Public License as published by
